steel/Zeta.Steel.LogEntry.fsti
@@ -8,3 +8,5 @@ val parser_log_entry : parser spec_parser_log_entry
 val serialize_stamped_record : serializer spec_serializer_stamped_record
 
 val serialize_value : serializer spec_serializer_value
+
+val parser_u256 : parser spec_parser_u256
